Launchbury/ArityAnalysisSig.thy
@@ -4,21 +4,5 @@ begin
 
 locale ArityAnalysis =
   fixes Aexp :: "exp \<Rightarrow> Arity \<rightarrow> AEnv"
-begin
-
-definition Aexp' :: "exp \<Rightarrow> Arity\<^sub>\<bottom> \<rightarrow> AEnv"
-  where "Aexp' e = fup \<cdot> (Aexp e)"
-
-lemma Aexp'_simps[simp]:
-  "Aexp' e \<cdot> \<bottom> = \<bottom>"
-  "Aexp' e \<cdot> (up\<cdot>n) = Aexp e \<cdot> n"
-  unfolding Aexp'_def by simp_all
-
-end
-
-lemma Aexp'_eqvt[eqvt]: "\<pi> \<bullet> (ArityAnalysis.Aexp' Aexp e) = ArityAnalysis.Aexp' (\<pi> \<bullet> Aexp) (\<pi> \<bullet> e)"
-  unfolding ArityAnalysis.Aexp'_def
-  by perm_simp rule
-
 
 end
