Launchbury/TrivialArityAnal.thy
@@ -61,12 +61,12 @@ lemma Trivial_Aheap_eqvt[eqvt]: "\<pi> \<bullet>  (Trivial_Aheap \<Gamma> e) = T
 lemma Trivial_Aheap_simp: "Trivial_Aheap \<Gamma> e\<cdot> a = (\<lambda> x. up\<cdot>0) f|` domA \<Gamma>"
   unfolding Trivial_Aheap_def by simp
 
-lemma Trivial_Aexp'_below_fv: "Aexp' e\<cdot>a \<sqsubseteq> (\<lambda> x . up\<cdot>0) f|` fv e"
+lemma Trivial_fup_Aexp_below_fv: "fup\<cdot>(Trivial_Aexp e)\<cdot>a \<sqsubseteq> (\<lambda> x . up\<cdot>0) f|` fv e"
   by (cases a)(auto simp add: Trivial_Aexp_simp)
 
 lemma Trivial_Abinds_below_fv: "ABinds \<Gamma>\<cdot>ae \<sqsubseteq> (\<lambda> x . up\<cdot>0) f|` fv \<Gamma>"
   by (induction \<Gamma> rule:ABinds.induct)
-     (auto simp add: join_below_iff intro!: below_trans[OF Trivial_Aexp'_below_fv] env_restr_mono2 elim: below_trans dest: set_mp[OF fv_delete_subset] simp del: fun_meet_simp)
+     (auto simp add: join_below_iff intro!: below_trans[OF Trivial_fup_Aexp_below_fv] env_restr_mono2 elim: below_trans dest: set_mp[OF fv_delete_subset] simp del: fun_meet_simp)
 
 interpretation CorrectArityAnalysisLet Trivial_Aexp Trivial_Aheap
 proof default
